IProofMode

proofmode/HSim.v
@@ -35,19 +35,6 @@ Section SIM.
   Variable stb: gname -> option fspec.
   Variable o: ord.
 
-  Variant fn_has_spec (fn: gname)
-          (pre: Any.t -> Any.t -> iProp)
-          (post: Any.t -> Any.t -> iProp)
-          (tbr: bool): Prop :=
-  | fn_has_spec_intro
-      fsp (x: fsp.(meta))
-      (STB: stb fn = Some fsp)
-      (MEASURE: ord_lt (fsp.(measure) x) o)
-      (PRE: forall arg_src arg_tgt, bi_entails (pre arg_src arg_tgt) (#=> fsp.(precond) (Some mn) x arg_src arg_tgt))
-      (POST: forall ret_src ret_tgt, bi_entails (fsp.(postcond) (Some mn) x ret_src ret_tgt: iProp) (#=> post ret_src ret_tgt))
-      (TBR: tbr = is_pure (fsp.(measure) x))
-  .
-
   Definition option_Ord_lt (o0 o1: option Ord.t): Prop :=
     match o0, o1 with
     | None, Some _ => True
@@ -109,6 +96,25 @@ Section SIM.
     destruct o0, o1, o2; ss. eapply Ord.le_lt_lt; eauto.
   Qed.
 
+  Definition inv_with w0 st_src st_tgt: iProp :=
+    (∃ w1, I w1 st_src st_tgt ** ⌜le w0 w1⌝)%I.
+
+  Lemma inv_with_current `{PreOrder _ le} w0 st_src st_tgt
+    :
+      bi_entails (I w0 st_src st_tgt) (inv_with w0 st_src st_tgt).
+  Proof.
+    unfold inv_with. iIntros "H". iExists w0. iSplit; auto.
+  Qed.
+
+  Lemma inv_with_le `{PreOrder _ le} w0 w1 st_src st_tgt
+        (LE: le w0 w1)
+    :
+      bi_entails (inv_with w1 st_src st_tgt) (inv_with w0 st_src st_tgt).
+  Proof.
+    unfold inv_with. iIntros "H". iDestruct "H" as (w2) "[H0 %]".
+    iExists w2. iSplit; auto. iPureIntro. etrans; eauto.
+  Qed.
+
   Inductive _hsim
             (hsim: forall R_src R_tgt
                           (Q: Any.t -> Any.t -> R_src -> R_tgt -> iProp)
@@ -131,12 +137,11 @@ Section SIM.
       st_src0 st_tgt0 ktr_src ktr_tgt
       fuel f_src f_tgt
       (SPEC: stb fn = Some fsp)
-      (PRE: current_iProp ctx (FR ** I w0 st_src0 st_tgt0 ** fsp.(precond) (Some mn) x arg_src arg_tgt))
+      (PRE: current_iProp ctx (FR ** inv_with w0 st_src0 st_tgt0 ** fsp.(precond) (Some mn) x arg_src arg_tgt))
       (MEASURE: o = ord_top)
       (NPURE: fsp.(measure) x = ord_top)
-      (POST: forall ctx1 w1 st_src1 st_tgt1 ret_src ret_tgt
-                    (LE: le w0 w1)
-                    (ACC: current_iProp ctx1 (FR ** I w1 st_src1 st_tgt1 ** fsp.(postcond) (Some mn) x ret_src ret_tgt)),
+      (POST: forall ctx1 st_src1 st_tgt1 ret_src ret_tgt
+                    (ACC: current_iProp ctx1 (FR ** inv_with w0 st_src1 st_tgt1 ** fsp.(postcond) (Some mn) x ret_src ret_tgt)),
           hsim _ _ Q ctx1 None true true (st_src1, ktr_src ret_src) (st_tgt1, ktr_tgt ret_tgt))
     :
       _hsim hsim Q ctx fuel f_src f_tgt (st_src0, trigger (Call fn arg_src) >>= ktr_src) (st_tgt0, trigger (Call fn arg_tgt) >>= ktr_tgt)
@@ -153,14 +158,13 @@ Section SIM.
       st_src0 st_tgt0 itr_src ktr_tgt
       fuel0 f_src f_tgt
       (SPEC: stb fn = Some fsp)
-      (PRE: current_iProp ctx (FR ** I w0 st_src0 st_tgt0 ** fsp.(precond) (Some mn) x arg_src arg_tgt))
+      (PRE: current_iProp ctx (FR ** inv_with w0 st_src0 st_tgt0 ** fsp.(precond) (Some mn) x arg_src arg_tgt))
       (MEASURE: ord_lt (fsp.(measure) x) o)
       (PURE: is_pure (fsp.(measure) x))
       (POST: exists fuel1,
           (<<FUEL: Ord.lt fuel1 fuel0>>) /\
-          (<<SIM: forall ctx1 w1 st_src1 st_tgt1 ret_src ret_tgt
-                         (LE: le w0 w1)
-                         (ACC: current_iProp ctx1 (FR ** I w1 st_src1 st_tgt1 ** fsp.(postcond) (Some mn) x ret_src ret_tgt)),
+          (<<SIM: forall ctx1 st_src1 st_tgt1 ret_src ret_tgt
+                         (ACC: current_iProp ctx1 (FR ** inv_with w0 st_src1 st_tgt1 ** fsp.(postcond) (Some mn) x ret_src ret_tgt)),
               hsim _ _ Q ctx1 (Some fuel1) true true (st_src1, itr_src) (st_tgt1, ktr_tgt ret_tgt)>>))
     :
       _hsim hsim Q ctx (Some fuel0) f_src f_tgt (st_src0, itr_src) (st_tgt0, trigger (Call fn arg_tgt) >>= ktr_tgt)
@@ -265,12 +269,11 @@ Section SIM.
             st_src0 st_tgt0 ktr_src ktr_tgt
             fuel f_src f_tgt
             (SPEC: stb fn = Some fsp)
-            (PRE: current_iProp ctx (FR ** I w0 st_src0 st_tgt0 ** fsp.(precond) (Some mn) x arg_src arg_tgt))
+            (PRE: current_iProp ctx (FR ** inv_with w0 st_src0 st_tgt0 ** fsp.(precond) (Some mn) x arg_src arg_tgt))
             (MEASURE: o = ord_top)
             (NPURE: fsp.(measure) x = ord_top)
-            (POST: forall ctx1 w1 st_src1 st_tgt1 ret_src ret_tgt
-                          (LE: le w0 w1)
-                          (ACC: current_iProp ctx1 (FR ** I w1 st_src1 st_tgt1 ** fsp.(postcond) (Some mn) x ret_src ret_tgt)),
+            (POST: forall ctx1 st_src1 st_tgt1 ret_src ret_tgt
+                          (ACC: current_iProp ctx1 (FR ** inv_with w0 st_src1 st_tgt1 ** fsp.(postcond) (Some mn) x ret_src ret_tgt)),
                 hsim _ _ Q ctx1 None true true (st_src1, ktr_src ret_src) (st_tgt1, ktr_tgt ret_tgt)),
             P fuel f_src f_tgt (st_src0, trigger (Call fn arg_src) >>= ktr_src) (st_tgt0, trigger (Call fn arg_tgt) >>= ktr_tgt))
         (APCSTART: forall
@@ -286,14 +289,13 @@ Section SIM.
             st_src0 st_tgt0 itr_src ktr_tgt
             fuel0 f_src f_tgt
             (SPEC: stb fn = Some fsp)
-            (PRE: current_iProp ctx (FR ** I w0 st_src0 st_tgt0 ** fsp.(precond) (Some mn) x arg_src arg_tgt))
+            (PRE: current_iProp ctx (FR ** inv_with w0 st_src0 st_tgt0 ** fsp.(precond) (Some mn) x arg_src arg_tgt))
             (MEASURE: ord_lt (fsp.(measure) x) o)
             (PURE: is_pure (fsp.(measure) x))
             (POST: exists fuel1,
                 (<<FUEL: Ord.lt fuel1 fuel0>>) /\
-                (<<SIM: forall ctx1 w1 st_src1 st_tgt1 ret_src ret_tgt
-                               (LE: le w0 w1)
-                               (ACC: current_iProp ctx1 (FR ** I w1 st_src1 st_tgt1 ** fsp.(postcond) (Some mn) x ret_src ret_tgt)),
+                (<<SIM: forall ctx1 st_src1 st_tgt1 ret_src ret_tgt
+                               (ACC: current_iProp ctx1 (FR ** inv_with w0 st_src1 st_tgt1 ** fsp.(postcond) (Some mn) x ret_src ret_tgt)),
                     hsim _ _ Q ctx1 (Some fuel1) true true (st_src1, itr_src) (st_tgt1, ktr_tgt ret_tgt)>>)),
             P (Some fuel0) f_src f_tgt (st_src0, itr_src) (st_tgt0, trigger (Call fn arg_tgt) >>= ktr_tgt))
         (SYSCALL: forall
@@ -435,12 +437,11 @@ Section SIM.
             st_src0 st_tgt0 ktr_src ktr_tgt
             fuel f_src f_tgt
             (SPEC: stb fn = Some fsp)
-            (PRE: current_iProp ctx (FR ** I w0 st_src0 st_tgt0 ** fsp.(precond) (Some mn) x arg_src arg_tgt))
+            (PRE: current_iProp ctx (FR ** inv_with w0 st_src0 st_tgt0 ** fsp.(precond) (Some mn) x arg_src arg_tgt))
             (MEASURE: o = ord_top)
             (NPURE: fsp.(measure) x = ord_top)
-            (POST: forall ctx1 w1 st_src1 st_tgt1 ret_src ret_tgt
-                          (LE: le w0 w1)
-                          (ACC: current_iProp ctx1 (FR ** I w1 st_src1 st_tgt1 ** fsp.(postcond) (Some mn) x ret_src ret_tgt)),
+            (POST: forall ctx1 st_src1 st_tgt1 ret_src ret_tgt
+                          (ACC: current_iProp ctx1 (FR ** inv_with w0 st_src1 st_tgt1 ** fsp.(postcond) (Some mn) x ret_src ret_tgt)),
                 hsim Q ctx1 None true true (st_src1, ktr_src ret_src) (st_tgt1, ktr_tgt ret_tgt)),
             P fuel f_src f_tgt (st_src0, trigger (Call fn arg_src) >>= ktr_src) (st_tgt0, trigger (Call fn arg_tgt) >>= ktr_tgt))
         (APCSTART: forall
@@ -456,14 +457,13 @@ Section SIM.
             st_src0 st_tgt0 itr_src ktr_tgt
             fuel0 f_src f_tgt
             (SPEC: stb fn = Some fsp)
-            (PRE: current_iProp ctx (FR ** I w0 st_src0 st_tgt0 ** fsp.(precond) (Some mn) x arg_src arg_tgt))
+            (PRE: current_iProp ctx (FR ** inv_with w0 st_src0 st_tgt0 ** fsp.(precond) (Some mn) x arg_src arg_tgt))
             (MEASURE: ord_lt (fsp.(measure) x) o)
             (PURE: is_pure (fsp.(measure) x))
             (POST: exists fuel1,
                 (<<FUEL: Ord.lt fuel1 fuel0>>) /\
-                (<<SIM: forall ctx1 w1 st_src1 st_tgt1 ret_src ret_tgt
-                               (LE: le w0 w1)
-                               (ACC: current_iProp ctx1 (FR ** I w1 st_src1 st_tgt1 ** fsp.(postcond) (Some mn) x ret_src ret_tgt)),
+                (<<SIM: forall ctx1 st_src1 st_tgt1 ret_src ret_tgt
+                               (ACC: current_iProp ctx1 (FR ** inv_with w0 st_src1 st_tgt1 ** fsp.(postcond) (Some mn) x ret_src ret_tgt)),
                     hsim Q ctx1 (Some fuel1) true true (st_src1, itr_src) (st_tgt1, ktr_tgt ret_tgt)>>)),
             P (Some fuel0) f_src f_tgt (st_src0, itr_src) (st_tgt0, trigger (Call fn arg_tgt) >>= ktr_tgt))
         (SYSCALL: forall
@@ -587,11 +587,11 @@ Section SIM.
     eapply current_iProp_entail; eauto.
   Qed.
 
-  Lemma hsim_adequacy_aux:
+  Lemma hsim_adequacy_aux `{PreOrder _ le}:
     forall
       f_src f_tgt st_src st_tgt (itr_src: itree (hAPCE +' Es) Any.t) itr_tgt mr_src ctx X (x: X) Q mn_caller fuel w0
       (SIM: hsim (fun st_src st_tgt ret_src ret_tgt =>
-                    (∃ w1, ⌜le w0 w1⌝ ** I w1 st_src st_tgt) ** (Q mn_caller x ret_src ret_tgt: iProp)) ctx fuel f_src f_tgt (st_src, itr_src) (st_tgt, itr_tgt)),
+                    (inv_with w0 st_src st_tgt) ** (Q mn_caller x ret_src ret_tgt: iProp)) ctx fuel f_src f_tgt (st_src, itr_src) (st_tgt, itr_tgt)),
       paco8 (_sim_itree (mk_wf I) le) bot8 Any.t Any.t (lift_rel (mk_wf I) le w0 (@eq Any.t))
             f_src f_tgt w0
             (Any.pair st_src mr_src,
@@ -603,29 +603,34 @@ Section SIM.
     revert st_src st_tgt itr_src itr_tgt Heqp Heqp0 CIH.
     induction SIM using hsim_ind; i; clarify.
     { eapply current_iPropL_convert in RET. mDesAll. destruct fuel; steps.
-      { astop. steps. hret _; eauto. iModIntro. iSplitL "A1"; auto. }
-      { hret _; eauto. iModIntro. iSplitL "A1"; auto. }
+      { astop. steps. unfold inv_with in RET. mDesAll. hret _; eauto.
+        iModIntro. iSplitL "H"; auto.
+      }
+      { unfold inv_with in RET. mDesAll. hret _; eauto.
+        iModIntro. iSplitL "H"; auto. }
     }
     { eapply current_iPropL_convert in PRE. mDesAll. destruct fuel; steps.
-      { astop. steps. rewrite SPEC. steps. destruct fsp. ss. hcall _ _ with "A A1".
+      { astop. steps. rewrite SPEC. steps. destruct fsp. ss.
+        unfold inv_with in PRE. mDesAll. hcall _ _ with "A A1".
         { iModIntro. iSplitL "A1"; eauto. iApply "A". }
         { rewrite MEASURE in *. splits; ss. unfold ord_lt. des_ifs. }
         { steps. gbase. hexploit CIH.
-          { eapply POST; [eauto|]. eapply current_iProp_entail; [eauto|].
+          { eapply POST. eapply current_iProp_entail; [eauto|].
             start_ipm_proof. iSplitR "POST".
-            { iSplitL "H"; eauto. }
+            { iSplitL "H"; eauto. iExists a1. iSplit; eauto. iPureIntro. etrans; eauto. }
             { iApply "POST". }
           }
           i. ss. eauto.
         }
       }
-      { rewrite SPEC. steps. destruct fsp. ss. hcall _ _ with "A A1".
+      { rewrite SPEC. steps. destruct fsp. ss.
+        unfold inv_with in PRE. mDesAll. hcall _ _ with "A A1".
         { iModIntro. iSplitL "A1"; eauto. iApply "A". }
         { rewrite MEASURE in *. splits; ss. unfold ord_lt. des_ifs. }
         { steps. gbase. hexploit CIH.
-          { eapply POST; [eauto|]. eapply current_iProp_entail; [eauto|].
+          { eapply POST. eapply current_iProp_entail; [eauto|].
             start_ipm_proof. iSplitR "POST".
-            { iSplitL "H"; eauto. }
+            { iSplitL "H"; eauto. iExists a1. iSplit; eauto. iPureIntro. etrans; eauto. }
             { iApply "POST". }
           }
           i. ss. eauto.
@@ -667,13 +672,14 @@ Section SIM.
       force_l. exists (fn, arg_src). steps.
       rewrite SPEC. steps.
       eapply current_iPropL_convert in PRE. mDesAll.
-      destruct fsp. ss. hcall _ _ with "A A1".
+      destruct fsp. ss. unfold inv_with in PRE. mDesAll.
+      hcall _ _ with "A A1".
       { iModIntro. iSplitL "A1"; eauto. iApply "A". }
       { splits; ss. }
       { steps. gbase. hexploit CIH.
-        { eapply SIM; [eauto|]. eapply current_iProp_entail; [eauto|].
+        { eapply SIM. eapply current_iProp_entail; [eauto|].
           start_ipm_proof. iSplitR "POST".
-          { iSplitL "H"; eauto. }
+          { iSplitL "H"; eauto. iExists a1. iSplit; eauto. iPureIntro. etrans; eauto. }
           { iApply "POST". }
         }
         i. ss. eauto.
@@ -711,11 +717,11 @@ Section SIM.
     { deflag. gbase. eapply CIH; eauto. }
   Qed.
 
-  Lemma hsim_adequacy:
+  Lemma hsim_adequacy `{PreOrder _ le}:
     forall
       f_src f_tgt st_src st_tgt (itr_src: itree (hAPCE +' Es) Any.t) itr_tgt mr_src ctx X (x: X) Q mn_caller w0
       (SIM: hsim (fun st_src st_tgt ret_src ret_tgt =>
-                    (∃ w1, ⌜le w0 w1⌝ ** I w1 st_src st_tgt) ** (Q mn_caller x ret_src ret_tgt: iProp)) ctx None f_src f_tgt (st_src, itr_src) (st_tgt, itr_tgt)),
+                    (inv_with w0 st_src st_tgt) ** (Q mn_caller x ret_src ret_tgt: iProp)) ctx None f_src f_tgt (st_src, itr_src) (st_tgt, itr_tgt)),
       paco8 (_sim_itree (mk_wf I) le) bot8 Any.t Any.t (lift_rel (mk_wf I) le w0 (@eq Any.t))
             f_src f_tgt w0
             (Any.pair st_src mr_src,
@@ -902,12 +908,11 @@ Section SIM.
       st_src0 st_tgt0 ktr_src ktr_tgt
       fuel f_src f_tgt
       (SPEC: stb fn = Some fsp)
-      (PRE: current_iProp ctx (FR ** I w0 st_src0 st_tgt0 ** fsp.(precond) (Some mn) x arg_src arg_tgt))
+      (PRE: current_iProp ctx (FR ** inv_with w0 st_src0 st_tgt0 ** fsp.(precond) (Some mn) x arg_src arg_tgt))
       (MEASURE: o = ord_top)
       (NPURE: fsp.(measure) x = ord_top)
-      (POST: forall ctx1 w1 st_src1 st_tgt1 ret_src ret_tgt
-                    (LE: le w0 w1)
-                    (ACC: current_iProp ctx1 (FR ** I w1 st_src1 st_tgt1 ** fsp.(postcond) (Some mn) x ret_src ret_tgt)),
+      (POST: forall ctx1 st_src1 st_tgt1 ret_src ret_tgt
+                    (ACC: current_iProp ctx1 (FR ** inv_with w0 st_src1 st_tgt1 ** fsp.(postcond) (Some mn) x ret_src ret_tgt)),
           g _ _ Q ctx1 None true true (st_src1, ktr_src ret_src) (st_tgt1, ktr_tgt ret_tgt))
     :
       hsimC r g Q ctx fuel f_src f_tgt (st_src0, trigger (Call fn arg_src) >>= ktr_src) (st_tgt0, trigger (Call fn arg_tgt) >>= ktr_tgt)
@@ -924,14 +929,13 @@ Section SIM.
       st_src0 st_tgt0 itr_src ktr_tgt
       fuel0 f_src f_tgt
       (SPEC: stb fn = Some fsp)
-      (PRE: current_iProp ctx (FR ** I w0 st_src0 st_tgt0 ** fsp.(precond) (Some mn) x arg_src arg_tgt))
+      (PRE: current_iProp ctx (FR ** inv_with w0 st_src0 st_tgt0 ** fsp.(precond) (Some mn) x arg_src arg_tgt))
       (MEASURE: ord_lt (fsp.(measure) x) o)
       (PURE: is_pure (fsp.(measure) x))
       (POST: exists fuel1,
           (<<FUEL: Ord.lt fuel1 fuel0>>) /\
-          (<<SIM: forall ctx1 w1 st_src1 st_tgt1 ret_src ret_tgt
-                         (LE: le w0 w1)
-                         (ACC: current_iProp ctx1 (FR ** I w1 st_src1 st_tgt1 ** fsp.(postcond) (Some mn) x ret_src ret_tgt)),
+          (<<SIM: forall ctx1 w0 st_src1 st_tgt1 ret_src ret_tgt
+                         (ACC: current_iProp ctx1 (FR ** inv_with w0 st_src1 st_tgt1 ** fsp.(postcond) (Some mn) x ret_src ret_tgt)),
               g _ _ Q ctx1 (Some fuel1) true true (st_src1, itr_src) (st_tgt1, ktr_tgt ret_tgt)>>))
     :
       hsimC r g Q ctx (Some fuel0) f_src f_tgt (st_src0, itr_src) (st_tgt0, trigger (Call fn arg_tgt) >>= ktr_tgt)
@@ -1493,878 +1497,6 @@ Section SIM.
         eapply URA.wf_mon. instantiate (1:=ctx0). r_wf H0.
       }
     }
-  Qed.
-
-  Definition back
-             (r g: forall R_src R_tgt
-                          (Q: Any.t -> Any.t -> R_src -> R_tgt -> iProp)
-                          (ctx: Σ),
-                 option Ord.t -> bool -> bool -> Any.t * itree hEs R_src -> Any.t * itree Es R_tgt -> Prop)
-             {R_src R_tgt}
-             (Q: Any.t -> Any.t -> R_src -> R_tgt -> iProp)
-             (fuel: option Ord.t)
-             (f_src f_tgt: bool)
-             (st_src: Any.t * itree hEs R_src)
-             (st_tgt: Any.t * itree Es R_tgt): iProp :=
-    fun res =>
-      forall ctx (WF: URA.wf (res ⋅ ctx)),
-        gpaco9 (_hsim) (cpn9 _hsim) r g _ _ Q ctx fuel f_src f_tgt st_src st_tgt.
-
-  Lemma back_init
-        R_src R_tgt (Q: Any.t -> Any.t -> R_src -> R_tgt -> iProp)
-        P r g ctx fuel f_src f_tgt st_src st_tgt itr_src itr_tgt
-        (ENTAIL: bi_entails
-                   P
-                   (back r g Q fuel f_src f_tgt (st_src, itr_src) (st_tgt, itr_tgt)))
-        (CUR: current_iProp ctx P)
-    :
-      gpaco9 _hsim (cpn9 _hsim) r g _ _ Q ctx fuel f_src f_tgt (st_src, itr_src) (st_tgt, itr_tgt).
-  Proof.
-    eapply current_iProp_entail in ENTAIL; eauto.
-    inv ENTAIL. unfold back in IPROP. eapply IPROP; eauto.
-  Qed.
-
-  Lemma back_final
-        R_src R_tgt (Q: Any.t -> Any.t -> R_src -> R_tgt -> iProp)
-        P r g fuel f_src f_tgt st_src st_tgt itr_src itr_tgt
-        (SIM: forall ctx
-                     (CUR: current_iProp ctx P),
-            gpaco9 _hsim (cpn9 _hsim) r g _ _ Q ctx fuel f_src f_tgt (st_src, itr_src) (st_tgt, itr_tgt))
-    :
-      bi_entails
-        P
-        (back r g Q fuel f_src f_tgt (st_src, itr_src) (st_tgt, itr_tgt)).
-  Proof.
-    uipropall. ii. eapply SIM. econs; eauto.
-  Qed.
-
-  Lemma back_current
-        R_src R_tgt (Q: Any.t -> Any.t -> R_src -> R_tgt -> iProp)
-        r g fuel ctx f_src f_tgt st_src st_tgt itr_src itr_tgt
-        (CUR: current_iProp ctx (back r g Q fuel f_src f_tgt (st_src, itr_src) (st_tgt, itr_tgt)))
-    :
-      gpaco9 _hsim (cpn9 _hsim) r g _ _ Q ctx fuel f_src f_tgt (st_src, itr_src) (st_tgt, itr_tgt).
-  Proof.
-    inv CUR. eapply IPROP; eauto.
-  Qed.
-
-  Lemma back_mono R_src R_tgt
-        (Q0 Q1: Any.t -> Any.t -> R_src -> R_tgt -> iProp)
-        r g fuel f_src f_tgt st_src itr_src st_tgt itr_tgt
-        (MONO: forall st_src st_tgt ret_src ret_tgt,
-            (bi_entails (Q0 st_src st_tgt ret_src ret_tgt) (#=> Q1 st_src st_tgt ret_src ret_tgt)))
-    :
-      bi_entails
-        (back r g Q0 fuel f_src f_tgt (st_src, itr_src) (st_tgt, itr_tgt))
-        (back r g Q1 fuel f_src f_tgt (st_src, itr_src) (st_tgt, itr_tgt)).
-  Proof.
-    red. unfold Entails. autorewrite with iprop.
-    unfold back in *. i. hexploit H; eauto. i.
-    guclo hmonoC_spec. econs; eauto.
-  Qed.
-
-  Lemma back_wand R_src R_tgt
-        (Q0 Q1: Any.t -> Any.t -> R_src -> R_tgt -> iProp)
-        r g fuel f_src f_tgt st_src itr_src st_tgt itr_tgt
-    :
-      bi_entails
-        ((∀ st_src st_tgt ret_src ret_tgt,
-             ((Q0 st_src st_tgt ret_src ret_tgt) -∗ (#=> Q1 st_src st_tgt ret_src ret_tgt))) ** (back r g Q0 fuel f_src f_tgt (st_src, itr_src) (st_tgt, itr_tgt)))
-        (back r g Q1 fuel f_src f_tgt (st_src, itr_src) (st_tgt, itr_tgt)).
-  Proof.
-    red. unfold Entails. autorewrite with iprop.
-    unfold back in *. i.
-    red in H. unfold Sepconj in H. autorewrite with iprop in H.
-    des. clarify. eapply from_semantic in H0. hexploit (H1 (ctx ⋅ a)).
-    { r_wf WF0. }
-    i. guclo hframeC_aux_spec. econs.
-    { instantiate (1:=a). eapply URA.wf_mon. instantiate (1:=b). r_wf WF0. }
-    guclo hmonoC_spec. econs.
-    { eapply H. }
-    i. iIntros "H0". iModIntro. iIntros "H1".
-    iPoseProof (H0 with "H1") as "H1".
-    iMod "H1". iApply "H1". iApply "H0".
-  Qed.
-
-  Lemma back_upd R_src R_tgt
-        (Q: Any.t -> Any.t -> R_src -> R_tgt -> iProp)
-        r g fuel f_src f_tgt st_src st_tgt
-    :
-      bi_entails
-        (#=> (back r g Q fuel f_src f_tgt st_src st_tgt))
-        (back r g Q fuel f_src f_tgt st_src st_tgt).
-  Proof.
-    red. unfold Entails. autorewrite with iprop.
-    unfold back in *. i.
-    red in H. unfold bi_bupd_bupd in H. ss. unfold Upd in H. autorewrite with iprop in H.
-    hexploit H; eauto. i. des.
-    hexploit H1; eauto.
-  Qed.
-
-  Lemma back_bind R_src R_tgt S_src S_tgt
-        (Q: Any.t -> Any.t -> R_src -> R_tgt -> iProp)
-        r g fuel f_src f_tgt st_src (itr_src: itree hEs S_src)
-        ktr_src st_tgt (itr_tgt: itree Es S_tgt) ktr_tgt
-    :
-      bi_entails
-        (back r g (fun st_src st_tgt ret_src ret_tgt => back r g Q None false false (st_src, ktr_src ret_src) (st_tgt, ktr_tgt ret_tgt)) fuel f_src f_tgt (st_src, itr_src) (st_tgt, itr_tgt))
-        (back r g Q fuel f_src f_tgt (st_src, itr_src >>= ktr_src) (st_tgt, itr_tgt >>= ktr_tgt)).
-  Proof.
-    red. unfold Entails. autorewrite with iprop.
-    unfold back in *. i.
-    guclo hbindC_spec. econs.
-    { eapply H; eauto. }
-    i. inv POST. eapply IPROP. eauto.
-  Qed.
-
-  Lemma back_bind_left R_src R_tgt S_src
-        (Q: Any.t -> Any.t -> R_src -> R_tgt -> iProp)
-        r g fuel f_src f_tgt st_src (itr_src: itree hEs S_src)
-        ktr_src st_tgt itr_tgt
-    :
-      bi_entails
-        (back r g (fun st_src st_tgt ret_src ret_tgt => back r g Q None false false (st_src, ktr_src ret_src) (st_tgt, itr_tgt)) fuel f_src f_tgt (st_src, itr_src) (st_tgt, Ret tt))
-        (back r g Q fuel f_src f_tgt (st_src, itr_src >>= ktr_src) (st_tgt, itr_tgt)).
-  Proof.
-    iIntros "H".
-    assert (EQ: itr_tgt = Ret tt >>= fun _ => itr_tgt).
-    { grind. }
-    rewrite EQ. iApply back_bind. rewrite <- EQ. iApply "H".
-  Qed.
-
-  Lemma back_bind_right R_src R_tgt S_tgt
-        (Q: Any.t -> Any.t -> R_src -> R_tgt -> iProp)
-        r g fuel f_src f_tgt st_src itr_src
-        st_tgt (itr_tgt: itree Es S_tgt) ktr_tgt
-    :
-      bi_entails
-        (back r g (fun st_src st_tgt ret_src ret_tgt => back r g Q None false false (st_src, itr_src) (st_tgt, ktr_tgt ret_tgt)) fuel f_src f_tgt (st_src, Ret tt) (st_tgt, itr_tgt))
-        (back r g Q fuel f_src f_tgt (st_src, itr_src) (st_tgt, itr_tgt >>= ktr_tgt)).
-  Proof.
-    iIntros "H".
-    assert (EQ: itr_src = Ret tt >>= fun _ => itr_src).
-    { grind. }
-    rewrite EQ. iApply back_bind. rewrite <- EQ. iApply "H".
-  Qed.
-
-  Lemma back_bind_right_pure R_src R_tgt S_tgt
-        (Q: Any.t -> Any.t -> R_src -> R_tgt -> iProp)
-        r g fuel f_src f_tgt st_src itr_src
-        st_tgt (itr_tgt: itree Es S_tgt) ktr_tgt
-    :
-      bi_entails
-        (back r g (fun st_src st_tgt ret_src ret_tgt => back r g Q fuel false false (st_src, itr_src) (st_tgt, ktr_tgt ret_tgt)) None f_src f_tgt (st_src, Ret tt) (st_tgt, itr_tgt))
-        (back r g Q fuel f_src f_tgt (st_src, itr_src) (st_tgt, itr_tgt >>= ktr_tgt)).
-  Proof.
-    red. unfold Entails. autorewrite with iprop.
-    unfold back in *. i.
-    guclo hbind_rightC_spec. econs.
-    { eapply H; eauto. }
-    i. inv POST. eapply IPROP. eauto.
-  Qed.
-
-  Lemma back_progress R_src R_tgt
-        (Q: Any.t -> Any.t -> R_src -> R_tgt -> iProp)
-        r g fuel st_src itr_src st_tgt itr_tgt
-    :
-      bi_entails
-        (back g g Q fuel false false (st_src, itr_src) (st_tgt, itr_tgt))
-        (back r g Q fuel true true (st_src, itr_src) (st_tgt, itr_tgt)).
-  Proof.
-    eapply back_final. i. eapply back_current in CUR.
-    eapply hsim_progress_flag. auto.
-  Qed.
-
-  Lemma back_flag_mon
-        fuel0 f_src0 f_tgt0
-        R_src R_tgt
-        (Q: Any.t -> Any.t -> R_src -> R_tgt -> iProp)
-        r g st_src itr_src st_tgt itr_tgt
-        fuel1 f_src1 f_tgt1
-        (SRC: f_src0 = true -> f_src1 = true)
-        (TGT: f_tgt0 = true -> f_tgt1 = true)
-        (FUEL: option_Ord_le fuel0 fuel1)
-    :
-      bi_entails
-        (back r g Q fuel0 f_src0 f_tgt0 (st_src, itr_src) (st_tgt, itr_tgt))
-        (back r g Q fuel1 f_src1 f_tgt1 (st_src, itr_src) (st_tgt, itr_tgt)).
-  Proof.
-    eapply back_final. i. eapply back_current in CUR.
-    guclo hflagC_spec. econs; eauto.
-  Qed.
-
-  Lemma back_split_aux R_src R_tgt S_tgt
-        (Q: Any.t -> Any.t -> R_src -> R_tgt -> iProp)
-        r g st_src itr_src st_tgt (itr_tgt: itree Es S_tgt) ktr_tgt
-        fuel0 fuel1 f_src f_tgt
-    :
-      bi_entails
-        (back r g (fun st_src st_tgt _ ret_tgt => back r g Q (Some fuel1) false false (st_src, itr_src) (st_tgt, ktr_tgt ret_tgt)) (Some fuel0) f_src f_tgt (st_src, Ret tt) (st_tgt, itr_tgt))
-        (back r g Q (Some (fuel1 + fuel0)%ord) f_src f_tgt (st_src, itr_src) (st_tgt, itr_tgt >>= ktr_tgt)).
-  Proof.
-    red. unfold Entails. autorewrite with iprop.
-    unfold back in *. i.
-    guclo hsplitC_spec. econs.
-    { eapply H; eauto. }
-    i. inv POST. eapply IPROP. eauto.
-  Qed.
-
-  Lemma back_split
-        fuel0 fuel1
-        R_src R_tgt S_tgt
-        (Q: Any.t -> Any.t -> R_src -> R_tgt -> iProp)
-        r g st_src itr_src st_tgt (itr_tgt: itree Es S_tgt) ktr_tgt
-        fuel f_src f_tgt
-        (FUEL: (fuel1 + fuel0 <= fuel)%ord)
-    :
-      bi_entails
-        (back r g (fun st_src st_tgt _ ret_tgt => back r g Q (Some fuel1) false false (st_src, itr_src) (st_tgt, ktr_tgt ret_tgt)) (Some fuel0) f_src f_tgt (st_src, Ret tt) (st_tgt, itr_tgt))
-        (back r g Q (Some fuel) f_src f_tgt (st_src, itr_src) (st_tgt, itr_tgt >>= ktr_tgt)).
-  Proof.
-    iIntros "H".
-    iApply back_flag_mon.
-    { eauto. }
-    { eauto. }
-    { instantiate (1:=Some (fuel1 + fuel0)%ord). ss. }
-    iApply back_split_aux. auto.
-  Qed.
-
-  Lemma back_call_impure
-        pre post w0
-        R_src R_tgt
-        (Q: Any.t -> Any.t -> R_src -> R_tgt -> iProp)
-        r g fuel f_src f_tgt st_src st_tgt fn arg_src arg_tgt ktr_src ktr_tgt
-        (SPEC: fn_has_spec fn pre post false)
-    :
-      bi_entails
-        ((#=> ((pre arg_src arg_tgt: iProp) ** I w0 st_src st_tgt))
-           **
-           (∀ st_src st_tgt ret_src ret_tgt,
-               ((∃ w1, I w1 st_src st_tgt ** ⌜le w0 w1⌝) ** (post ret_src ret_tgt: iProp)) -* #=> back g g Q None true true (st_src, ktr_src ret_src) (st_tgt, ktr_tgt ret_tgt)))
-        (back r g Q fuel f_src f_tgt (st_src, trigger (Call fn arg_src) >>= ktr_src) (st_tgt, trigger (Call fn arg_tgt) >>= ktr_tgt)).
-  Proof.
-    red. unfold Entails. autorewrite with iprop.
-    unfold back at 2. i.
-    match (type of H) with
-    | ?P _ =>
-      assert (CUR: current_iProp ctx P)
-    end.
-    { econs; eauto. }
-    apply current_iPropL_convert in CUR.
-    mDesAll. mUpd "H". mDesSep "H".
-    ired_both. gstep. inv SPEC. econs; eauto.
-    { mAssert _ with "H".
-      { iApply (PRE with "H"). }
-      mUpd "A2".
-      eapply current_iProp_entail; [eapply CUR|]. start_ipm_proof.
-      iSplitR "A2"; [|iExact "A2"].
-      iSplitR "A1"; [|iExact "A1"].
-      iExact "A".
-    }
-    { destruct (measure fsp x), o; ss. }
-    { destruct (measure fsp x), o; ss. }
-    i. apply current_iPropL_convert in ACC.
-    mDesAll. mSpcUniv "H" with st_src1.
-    mSpcUniv "H" with st_tgt1.
-    mSpcUniv "H" with ret_src.
-    mSpcUniv "H" with ret_tgt.
-    mAssert _ with "A".
-    { iApply (POST with "A"). }
-    mUpd "A2".
-    mAssert (#=> (back g g Q None true true (st_src1, ktr_src ret_src)
-                       (st_tgt1, ktr_tgt ret_tgt))) with "*".
-    { iApply "H". iSplitR "A2"; [|iExact "A2"].
-      iExists w1. iSplit; ss.
-    }
-    mUpd "A".
-    inv ACC. red in IPROP. uipropall. des. subst. eapply IPROP0.
-    eapply URA.wf_mon. instantiate (1:=b). r_wf GWF.
-  Qed.
-
-  Lemma back_call_pure
-        pre post w0 fuel1
-        R_src R_tgt
-        (Q: Any.t -> Any.t -> R_src -> R_tgt -> iProp)
-        r g f_src f_tgt st_src st_tgt fn arg_src arg_tgt itr_src ktr_tgt
-        fuel0
-        (SPEC: fn_has_spec fn pre post true)
-        (FUEL: Ord.lt fuel1 fuel0)
-    :
-      bi_entails
-        ((#=> ((pre arg_src arg_tgt: iProp) ** I w0 st_src st_tgt))
-           **
-           (∀ st_src st_tgt ret_src ret_tgt,
-               ((∃ w1, I w1 st_src st_tgt ** ⌜le w0 w1⌝) ** (post ret_src ret_tgt: iProp)) -* #=> back g g Q (Some fuel1) true true (st_src, itr_src) (st_tgt, ktr_tgt ret_tgt)))
-        (back r g Q (Some fuel0) f_src f_tgt (st_src, itr_src) (st_tgt, trigger (Call fn arg_tgt) >>= ktr_tgt)).
-  Proof.
-    red. unfold Entails. autorewrite with iprop.
-    unfold back at 2. i.
-    match (type of H) with
-    | ?P _ =>
-      assert (CUR: current_iProp ctx P)
-    end.
-    { econs; eauto. }
-    apply current_iPropL_convert in CUR.
-    mDesAll. mUpd "H". mDesSep "H".
-    ired_both. gstep. inv SPEC. econs; eauto.
-    { mAssert _ with "H".
-      { iApply (PRE with "H"). }
-      mUpd "A2".
-      eapply current_iProp_entail; [eapply CUR|]. start_ipm_proof.
-      iSplitR "A2"; [|iExact "A2"].
-      iSplitR "A1"; [|iExact "A1"].
-      iExact "A".
-    }
-    { destruct (measure fsp x), o; ss. }
-    esplits; eauto.
-    i. apply current_iPropL_convert in ACC.
-    mDesAll. mSpcUniv "H" with st_src1.
-    mSpcUniv "H" with st_tgt1.
-    mSpcUniv "H" with ret_src.
-    mSpcUniv "H" with ret_tgt.
-    mAssert _ with "A".
-    { iApply (POST with "A"). }
-    mUpd "A2".
-    mAssert (#=> back g g Q (Some fuel1) true true (st_src1, itr_src) (st_tgt1, ktr_tgt ret_tgt)) with "*".
-    { iApply "H". iSplitR "A2"; [|iExact "A2"].
-      iExists w1. iSplit; ss.
-    }
-    mUpd "A".
-    inv ACC. red in IPROP. uipropall. des. subst. eapply IPROP0.
-    eapply URA.wf_mon. instantiate (1:=b). r_wf GWF.
-  Qed.
-
-  Lemma back_ret
-        R_src R_tgt (Q: Any.t -> Any.t -> R_src -> R_tgt -> iProp)
-        r g
-        v_src v_tgt
-        st_src st_tgt
-        fuel f_src f_tgt
-    :
-      bi_entails
-        (#=> Q st_src st_tgt v_src v_tgt)
-        (back r g Q fuel f_src f_tgt (st_src, Ret v_src) (st_tgt, (Ret v_tgt))).
-  Proof.
-    eapply back_final. i. apply current_iProp_upd in CUR.
-    eapply hsimC_uclo. econs; eauto.
-  Qed.
-
-  Lemma back_apc
-        R_src R_tgt
-        (Q: Any.t -> Any.t -> R_src -> R_tgt -> iProp)
-        r g f_src f_tgt st_src st_tgt ktr_src itr_tgt
-        fuel0
-    :
-      bi_entails
-        (∃ fuel1, back r g Q fuel1 true f_tgt (st_src, ktr_src tt) (st_tgt, itr_tgt))
-        (back r g Q fuel0 f_src f_tgt (st_src, trigger hAPC >>= ktr_src) (st_tgt, itr_tgt)).
-  Proof.
-    eapply back_final. i.
-    inv CUR. red in IPROP. uipropall. des.
-    eapply hsimC_uclo. econs; eauto.
-  Qed.
-
-  Lemma back_apc_trigger
-        R_tgt
-        (Q: Any.t -> Any.t -> unit -> R_tgt -> iProp)
-        r g f_src f_tgt st_src st_tgt itr_tgt
-        fuel0
-    :
-      bi_entails
-        (∃ fuel1, back r g Q fuel1 true f_tgt (st_src, Ret tt) (st_tgt, itr_tgt))
-        (back r g Q fuel0 f_src f_tgt (st_src, trigger hAPC) (st_tgt, itr_tgt)).
-  Proof.
-    erewrite (@idK_spec _ _ (trigger (hAPC))).
-    iIntros "H". iApply back_apc. iExact "H".
-  Qed.
-
-  Lemma back_call_impure_trigger
-        pre post w0
-        (Q: Any.t -> Any.t -> Any.t -> Any.t -> iProp)
-        r g fuel f_src f_tgt st_src st_tgt fn arg_src arg_tgt
-        (SPEC: fn_has_spec fn pre post false)
-    :
-      bi_entails
-        ((#=> ((pre arg_src arg_tgt: iProp) ** I w0 st_src st_tgt))
-           **
-           (∀ st_src st_tgt ret_src ret_tgt,
-               ((∃ w1, I w1 st_src st_tgt ** ⌜le w0 w1⌝) ** (post ret_src ret_tgt: iProp)) -* #=> Q st_src st_tgt ret_src ret_tgt))
-        (back r g Q fuel f_src f_tgt (st_src, trigger (Call fn arg_src)) (st_tgt, trigger (Call fn arg_tgt))).
-  Proof.
-    erewrite (@idK_spec _ _ (trigger (Call fn arg_src))).
-    erewrite (@idK_spec _ _ (trigger (Call fn arg_tgt))).
-    iIntros "H". iApply back_call_impure; eauto.
-    iDestruct "H" as "[H0 H1]". iSplitL "H0"; auto.
-    iIntros (st_src0 st_tgt0 ret_src ret_tgt) "H".
-    iModIntro. iApply back_ret. iApply "H1". auto.
-  Qed.
-
-  Lemma back_call_pure_trigger
-        pre post w0
-        (Q: Any.t -> Any.t -> unit -> Any.t -> iProp)
-        r g f_src f_tgt st_src st_tgt fn arg_src arg_tgt
-        (SPEC: fn_has_spec fn pre post true)
-    :
-      bi_entails
-        ((#=> ((pre arg_src arg_tgt: iProp) ** I w0 st_src st_tgt))
-           **
-           (∀ st_src st_tgt ret_src ret_tgt,
-               ((∃ w1, I w1 st_src st_tgt ** ⌜le w0 w1⌝) ** (post ret_src ret_tgt: iProp)) -* #=> Q st_src st_tgt tt ret_tgt))
-        (back r g Q (Some (1: Ord.t)) f_src f_tgt (st_src, Ret tt) (st_tgt, trigger (Call fn arg_tgt))).
-  Proof.
-    erewrite (@idK_spec _ _ (trigger (Call fn arg_tgt))).
-    iIntros "H". iApply back_call_pure; eauto.
-    { oauto. }
-    iDestruct "H" as "[H0 H1]". iSplitL "H0"; auto.
-    iIntros (st_src0 st_tgt0 ret_src ret_tgt) "H".
-    iModIntro. iApply back_ret. iApply "H1". auto.
-  Qed.
-
-  Lemma back_syscall
-        R_src R_tgt
-        (Q: Any.t -> Any.t -> R_src -> R_tgt -> iProp)
-        fn arg rvs
-        r g fuel f_src f_tgt st_src st_tgt ktr_src ktr_tgt
-    :
-      bi_entails
-        (∀ ret, back g g Q None true true (st_src, ktr_src ret) (st_tgt, ktr_tgt ret))
-        (back r g Q fuel f_src f_tgt (st_src, trigger (Syscall fn arg rvs) >>= ktr_src) (st_tgt, trigger (Syscall fn arg rvs) >>= ktr_tgt)).
-  Proof.
-    eapply back_final. i. eapply hsimC_uclo. econs; eauto.
-    i. inv CUR. red in IPROP. uipropall. eapply IPROP; eauto.
-  Qed.
-
-  Global Instance iProp_back_absorbing
-         R_src R_tgt r g (Q: Any.t -> Any.t -> R_src -> R_tgt -> iProp)
-         fuel f_src f_tgt st_src st_tgt:
-    Absorbing (back r g Q fuel f_src f_tgt st_src st_tgt).
-  Proof.
-    unfold Absorbing. unfold bi_absorbingly.
-    iIntros "[H0 H1]". iApply back_upd.
-    iDestruct "H0" as "%". iModIntro. iApply "H1".
-  Qed.
-
-  Global Instance iProp_back_elim_upd
-         R_src R_tgt r g (Q: Any.t -> Any.t -> R_src -> R_tgt -> iProp)
-         fuel f_src f_tgt st_src st_tgt
-         P:
-    ElimModal True false false (#=> P) P (back r g Q fuel f_src f_tgt st_src st_tgt) (back r g Q fuel f_src f_tgt st_src st_tgt).
-  Proof.
-    unfold ElimModal. i. iIntros "[H0 H1]".
-    iApply back_upd. iMod "H0". iModIntro.
-    iApply "H1". iApply "H0".
-  Qed.
-
-  Lemma back_syscall_trigger
-        (Q: Any.t -> Any.t -> Any.t -> Any.t -> iProp)
-        fn arg_src arg_tgt rvs
-        r g fuel f_src f_tgt st_src st_tgt
-    :
-      bi_entails
-        (⌜arg_src = arg_tgt⌝ ** ∀ ret, Q st_src st_tgt ret ret)
-        (back r g Q fuel f_src f_tgt (st_src, trigger (Syscall fn arg_src rvs)) (st_tgt, trigger (Syscall fn arg_tgt rvs))).
-  Proof.
-    erewrite (@idK_spec _ _ (trigger (Syscall fn arg_src rvs))).
-    erewrite (@idK_spec _ _ (trigger (Syscall fn arg_tgt rvs))).
-    iIntros "[% H1]". subst.
-    iApply back_syscall. iIntros (ret).
-    iApply back_ret. iModIntro. iApply "H1".
-  Qed.
-
-  Lemma back_tau_src
-        R_src R_tgt
-        (Q: Any.t -> Any.t -> R_src -> R_tgt -> iProp)
-        r g fuel f_src f_tgt st_src st_tgt itr_src itr_tgt
-    :
-      bi_entails
-        (back r g Q None true f_tgt (st_src, itr_src) (st_tgt, itr_tgt))
-        (back r g Q fuel f_src f_tgt (st_src, tau;; itr_src) (st_tgt, itr_tgt)).
-  Proof.
-    eapply back_final. i. eapply hsimC_uclo. econs; eauto.
-    eapply back_current; eauto.
-  Qed.
-
-  Lemma back_tau_tgt
-        R_src R_tgt
-        (Q: Any.t -> Any.t -> R_src -> R_tgt -> iProp)
-        r g fuel f_src f_tgt st_src st_tgt itr_src itr_tgt
-    :
-      bi_entails
-        (back r g Q fuel f_src true (st_src, itr_src) (st_tgt, itr_tgt))
-        (back r g Q fuel f_src f_tgt (st_src, itr_src) (st_tgt, tau;; itr_tgt)).
-  Proof.
-    eapply back_final. i. eapply hsimC_uclo. econs; eauto.
-    eapply back_current; eauto.
-  Qed.
-
-  Lemma back_choose_src
-        R_src R_tgt
-        (Q: Any.t -> Any.t -> R_src -> R_tgt -> iProp)
-        r g fuel f_src f_tgt st_src st_tgt X ktr_src itr_tgt
-    :
-      bi_entails
-        (∃ x, back r g Q None true f_tgt (st_src, ktr_src x) (st_tgt, itr_tgt))
-        (back r g Q fuel f_src f_tgt (st_src, trigger (Choose X) >>= ktr_src) (st_tgt, itr_tgt)).
-  Proof.
-    eapply back_final. i. eapply hsimC_uclo. econs; eauto.
-    inv CUR. red in IPROP. uipropall. des. esplits. eapply IPROP; eauto.
-  Qed.
-
-  Lemma back_choose_src_trigger
-        X
-        (Q: Any.t -> Any.t -> X -> unit -> iProp)
-        r g fuel f_src f_tgt st_src st_tgt
-    :
-      bi_entails
-        (∃ x, Q st_src st_tgt x tt)
-        (back r g Q fuel f_src f_tgt (st_src, trigger (Choose X)) (st_tgt, Ret tt)).
-  Proof.
-    erewrite (@idK_spec _ _ (trigger (Choose X))).
-    iIntros "H". iApply back_choose_src.
-    iDestruct "H" as (x) "H". iExists x.
-    iApply back_ret. iModIntro. iApply "H".
-  Qed.
-
-  Lemma back_choose_tgt
-        R_src R_tgt
-        (Q: Any.t -> Any.t -> R_src -> R_tgt -> iProp)
-        r g fuel f_src f_tgt st_src st_tgt X itr_src ktr_tgt
-    :
-      bi_entails
-        (∀ x, back r g Q fuel f_src true (st_src, itr_src) (st_tgt, ktr_tgt x))
-        (back r g Q fuel f_src f_tgt (st_src, itr_src) (st_tgt, trigger (Choose X) >>= ktr_tgt)).
-  Proof.
-    eapply back_final. i. eapply hsimC_uclo. econs; eauto.
-    inv CUR. red in IPROP. uipropall. i. eapply IPROP; eauto.
-  Qed.
-
-  Lemma back_choose_tgt_trigger
-        X
-        (Q: Any.t -> Any.t -> unit -> X -> iProp)
-        r g fuel f_src f_tgt st_src st_tgt
-    :
-      bi_entails
-        (∀ x, Q st_src st_tgt tt x)
-        (back r g Q fuel f_src f_tgt (st_src, Ret tt) (st_tgt, trigger (Choose X))).
-  Proof.
-    erewrite (@idK_spec _ _ (trigger (Choose X))).
-    iIntros "H". iApply back_choose_tgt.
-    iIntros (x). iApply back_ret. iModIntro. iApply "H".
-  Qed.
-
-  Lemma back_take_src
-        R_src R_tgt
-        (Q: Any.t -> Any.t -> R_src -> R_tgt -> iProp)
-        r g fuel f_src f_tgt st_src st_tgt X ktr_src itr_tgt
-    :
-      bi_entails
-        (∀ x, back r g Q None true f_tgt (st_src, ktr_src x) (st_tgt, itr_tgt))
-        (back r g Q fuel f_src f_tgt (st_src, trigger (Take X) >>= ktr_src) (st_tgt, itr_tgt)).
-  Proof.
-    eapply back_final. i. eapply hsimC_uclo. econs; eauto.
-    inv CUR. red in IPROP. uipropall. i. eapply IPROP; eauto.
-  Qed.
-
-  Lemma back_take_src_trigger
-        X
-        (Q: Any.t -> Any.t -> X -> unit -> iProp)
-        r g fuel f_src f_tgt st_src st_tgt
-    :
-      bi_entails
-        (∀ x, Q st_src st_tgt x tt)
-        (back r g Q fuel f_src f_tgt (st_src, trigger (Take X)) (st_tgt, Ret tt)).
-  Proof.
-    erewrite (@idK_spec _ _ (trigger (Take X))).
-    iIntros "H". iApply back_take_src.
-    iIntros (x). iApply back_ret. iModIntro. iApply "H".
-  Qed.
-
-  Lemma back_take_tgt
-        R_src R_tgt
-        (Q: Any.t -> Any.t -> R_src -> R_tgt -> iProp)
-        r g fuel f_src f_tgt st_src st_tgt X itr_src ktr_tgt
-    :
-      bi_entails
-        (∃ x, back r g Q fuel f_src true (st_src, itr_src) (st_tgt, ktr_tgt x))
-        (back r g Q fuel f_src f_tgt (st_src, itr_src) (st_tgt, trigger (Take X) >>= ktr_tgt)).
-  Proof.
-    eapply back_final. i. eapply hsimC_uclo. econs; eauto.
-    inv CUR. red in IPROP. uipropall. des. esplits. eapply IPROP; eauto.
-  Qed.
-
-  Lemma back_take_tgt_trigger
-        X
-        (Q: Any.t -> Any.t -> unit -> X -> iProp)
-        r g fuel f_src f_tgt st_src st_tgt
-    :
-      bi_entails
-        (∃ x, Q st_src st_tgt tt x)
-        (back r g Q fuel f_src f_tgt (st_src, Ret tt) (st_tgt, trigger (Take X))).
-  Proof.
-    erewrite (@idK_spec _ _ (trigger (Take X))).
-    iIntros "H". iApply back_take_tgt.
-    iDestruct "H" as (x) "H". iExists x.
-    iApply back_ret. iModIntro. iApply "H".
-  Qed.
-
-  Lemma back_pput_src
-        R_src R_tgt
-        (Q: Any.t -> Any.t -> R_src -> R_tgt -> iProp)
-        r g fuel f_src f_tgt st_src0 st_src1 st_tgt ktr_src itr_tgt
-    :
-      bi_entails
-        (back r g Q None true f_tgt (st_src1, ktr_src tt) (st_tgt, itr_tgt))
-        (back r g Q fuel f_src f_tgt (st_src0, trigger (PPut st_src1) >>= ktr_src) (st_tgt, itr_tgt)).
-  Proof.
-    eapply back_final. i. eapply hsimC_uclo. econs; eauto.
-    eapply back_current; eauto.
-  Qed.
-
-  Lemma back_pput_src_trigger
-        (Q: Any.t -> Any.t -> unit -> unit -> iProp)
-        r g fuel f_src f_tgt st_src0 st_src1 st_tgt
-    :
-      bi_entails
-        (Q st_src1 st_tgt tt tt)
-        (back r g Q fuel f_src f_tgt (st_src0, trigger (PPut st_src1)) (st_tgt, Ret tt)).
-  Proof.
-    erewrite (@idK_spec _ _ (trigger (PPut st_src1))).
-    iIntros "H". iApply back_pput_src.
-    iApply back_ret. iModIntro. iApply "H".
-  Qed.
-
-  Lemma back_pget_src
-        R_src R_tgt
-        (Q: Any.t -> Any.t -> R_src -> R_tgt -> iProp)
-        r g fuel f_src f_tgt st_src st_tgt ktr_src itr_tgt
-    :
-      bi_entails
-        (back r g Q None true f_tgt (st_src, ktr_src st_src) (st_tgt, itr_tgt))
-        (back r g Q fuel f_src f_tgt (st_src, trigger (PGet) >>= ktr_src) (st_tgt, itr_tgt)).
-  Proof.
-    eapply back_final. i. eapply hsimC_uclo. econs; eauto.
-    eapply back_current; eauto.
-  Qed.
-
-  Lemma back_get_src_trigger
-        (Q: Any.t -> Any.t -> Any.t -> unit -> iProp)
-        r g fuel f_src f_tgt st_src st_tgt
-    :
-      bi_entails
-        (Q st_src st_tgt st_src tt)
-        (back r g Q fuel f_src f_tgt (st_src, trigger (PGet)) (st_tgt, Ret tt)).
-  Proof.
-    erewrite (@idK_spec _ _ (trigger (PGet))).
-    iIntros "H". iApply back_pget_src.
-    iApply back_ret. iModIntro. iApply "H".
-  Qed.
-
-  Lemma back_pput_tgt
-        R_src R_tgt
-        (Q: Any.t -> Any.t -> R_src -> R_tgt -> iProp)
-        r g fuel f_src f_tgt st_src st_tgt0 st_tgt1 itr_src ktr_tgt
-    :
-      bi_entails
-        (back r g Q fuel f_src true (st_src, itr_src) (st_tgt1, ktr_tgt tt))
-        (back r g Q fuel f_src f_tgt (st_src, itr_src) (st_tgt0, trigger (PPut st_tgt1) >>= ktr_tgt)).
-  Proof.
-    eapply back_final. i. eapply hsimC_uclo. econs; eauto.
-    eapply back_current; eauto.
-  Qed.
-
-  Lemma back_pput_tgt_trigger
-        (Q: Any.t -> Any.t -> unit -> unit -> iProp)
-        r g fuel f_src f_tgt st_src st_tgt0 st_tgt1
-    :
-      bi_entails
-        (Q st_src st_tgt1 tt tt)
-        (back r g Q fuel f_src f_tgt (st_src, Ret tt) (st_tgt0, trigger (PPut st_tgt1))).
-  Proof.
-    erewrite (@idK_spec _ _ (trigger (PPut st_tgt1))).
-    iIntros "H". iApply back_pput_tgt.
-    iApply back_ret. iModIntro. iApply "H".
-  Qed.
-
-  Lemma back_pget_tgt
-        R_src R_tgt
-        (Q: Any.t -> Any.t -> R_src -> R_tgt -> iProp)
-        r g fuel f_src f_tgt st_src st_tgt itr_src ktr_tgt
-    :
-      bi_entails
-        (back r g Q fuel f_src true (st_src, itr_src) (st_tgt, ktr_tgt st_tgt))
-        (back r g Q fuel f_src f_tgt (st_src, itr_src) (st_tgt, trigger (PGet) >>= ktr_tgt)).
-  Proof.
-    eapply back_final. i. eapply hsimC_uclo. econs; eauto.
-    eapply back_current; eauto.
-  Qed.
-
-  Lemma back_pget_tgt_trigger
-        (Q: Any.t -> Any.t -> unit -> Any.t -> iProp)
-        r g fuel f_src f_tgt st_src st_tgt
-    :
-      bi_entails
-        (Q st_src st_tgt tt st_tgt)
-        (back r g Q fuel f_src f_tgt (st_src, Ret tt) (st_tgt, trigger (PGet))).
-  Proof.
-    erewrite (@idK_spec _ _ (trigger (PGet))).
-    iIntros "H". iApply back_pget_tgt.
-    iApply back_ret. iModIntro. iApply "H".
-  Qed.
-
-  Lemma back_assume_src
-        (Q: Any.t -> Any.t -> unit -> unit -> iProp)
-        r g fuel f_src f_tgt st_src st_tgt P
-    :
-      bi_entails
-        (⌜P⌝ -* Q st_src st_tgt tt tt)
-        (back r g Q fuel f_src f_tgt (st_src, assume P) (st_tgt, Ret tt)).
-  Proof.
-    iIntros "H". unfold assume.
-    iApply back_bind_left. iApply back_take_src_trigger.
-    iIntros (H). iApply back_ret. iModIntro. iApply "H". iPureIntro. auto.
-  Qed.
-
-  Lemma back_assume_tgt
-        (Q: Any.t -> Any.t -> unit -> unit -> iProp)
-        r g fuel f_src f_tgt st_src st_tgt P
-    :
-      bi_entails
-        (⌜P⌝ ∧ Q st_src st_tgt tt tt)
-        (back r g Q fuel f_src f_tgt (st_src, Ret tt) (st_tgt, assume P)).
-  Proof.
-    iIntros "H". iDestruct "H" as "[% H]".
-    unfold assume. iApply back_bind_right. iApply back_take_tgt_trigger.
-    iExists H. iApply back_ret. iModIntro. iApply "H".
-  Qed.
-
-  Lemma back_guarantee_src
-        (Q: Any.t -> Any.t -> unit -> unit -> iProp)
-        r g fuel f_src f_tgt st_src st_tgt P
-    :
-      bi_entails
-        (⌜P⌝ ∧ Q st_src st_tgt tt tt)
-        (back r g Q fuel f_src f_tgt (st_src, guarantee P) (st_tgt, Ret tt)).
-  Proof.
-    iIntros "H". iDestruct "H" as "[% H]".
-    unfold guarantee. iApply back_bind_left. iApply back_choose_src_trigger.
-    iExists H. iApply back_ret. iModIntro. iApply "H".
-  Qed.
-
-  Lemma back_guarantee_tgt
-        (Q: Any.t -> Any.t -> unit -> unit -> iProp)
-        r g fuel f_src f_tgt st_src st_tgt P
-    :
-      bi_entails
-        (⌜P⌝ -* Q st_src st_tgt tt tt)
-        (back r g Q fuel f_src f_tgt (st_src, Ret tt) (st_tgt, guarantee P)).
-  Proof.
-    iIntros "H". unfold guarantee.
-    iApply back_bind_right. iApply back_choose_tgt_trigger.
-    iIntros (H). iApply back_ret. iModIntro. iApply "H". iPureIntro. auto.
-  Qed.
-
-  Lemma back_triggerUB_src
-        R_src R_tgt
-        (Q: Any.t -> Any.t -> R_src -> R_tgt -> iProp)
-        r g fuel f_src f_tgt st_src st_tgt itr_tgt
-    :
-      bi_entails
-        (⌜True⌝)
-        (back r g Q fuel f_src f_tgt (st_src, triggerUB) (st_tgt, itr_tgt)).
-  Proof.
-    iIntros "H". iApply back_take_src.
-    iIntros (x). destruct x.
-  Qed.
-
-  Lemma back_triggerNB_src
-        R_src R_tgt
-        (Q: Any.t -> Any.t -> R_src -> R_tgt -> iProp)
-        r g fuel f_src f_tgt st_src st_tgt itr_tgt
-    :
-      bi_entails
-        (⌜False⌝)
-        (back r g Q fuel f_src f_tgt (st_src, triggerUB) (st_tgt, itr_tgt)).
-  Proof.
-    iIntros "%". inv H.
-  Qed.
-
-  Lemma back_triggerUB_tgt
-        R_src R_tgt
-        (Q: Any.t -> Any.t -> R_src -> R_tgt -> iProp)
-        r g fuel f_src f_tgt st_src st_tgt itr_src
-    :
-      bi_entails
-        (⌜False⌝)
-        (back r g Q fuel f_src f_tgt (st_src, itr_src) (st_tgt, triggerUB)).
-  Proof.
-    iIntros "%". inv H.
-  Qed.
-
-  Lemma back_triggerNB_tgt
-        R_src R_tgt
-        (Q: Any.t -> Any.t -> R_src -> R_tgt -> iProp)
-        r g fuel f_src f_tgt st_src st_tgt itr_src
-    :
-      bi_entails
-        (⌜True⌝)
-        (back r g Q fuel f_src f_tgt (st_src, itr_src) (st_tgt, triggerNB)).
-  Proof.
-    iIntros "H". iApply back_choose_tgt.
-    iIntros (x). destruct x.
-  Qed.
-
-  Lemma back_unwrapU_src
-        X
-        (Q: Any.t -> Any.t -> X -> unit -> iProp)
-        r g fuel f_src f_tgt st_src st_tgt x
-    :
-      bi_entails
-        (∀ x', ⌜x = Some x'⌝ -* Q st_src st_tgt x' tt)
-        (back r g Q fuel f_src f_tgt (st_src, unwrapU x) (st_tgt, Ret tt)).
-  Proof.
-    iIntros "H". unfold unwrapU. destruct x.
-    { iApply back_ret. iModIntro. iApply "H". auto. }
-    { iApply back_triggerUB_src. auto. }
-  Qed.
-
-  Lemma back_unwrapN_src
-        X
-        (Q: Any.t -> Any.t -> X -> unit -> iProp)
-        r g fuel f_src f_tgt st_src st_tgt x
-    :
-      bi_entails
-        (∃ x', ⌜x = Some x'⌝ ∧ Q st_src st_tgt x' tt)
-        (back r g Q fuel f_src f_tgt (st_src, unwrapN x) (st_tgt, Ret tt)).
-  Proof.
-    iIntros "H". iDestruct "H" as (x') "[% H]". subst. ss.
-    iApply back_ret. iModIntro. iApply "H".
-  Qed.
-
-  Lemma back_unwrapU_tgt
-        X
-        (Q: Any.t -> Any.t -> unit -> X -> iProp)
-        r g fuel f_src f_tgt st_src st_tgt x
-    :
-      bi_entails
-        (∃ x', ⌜x = Some x'⌝ ∧ Q st_src st_tgt tt x')
-        (back r g Q fuel f_src f_tgt (st_src, Ret tt) (st_tgt, unwrapU x)).
-  Proof.
-    iIntros "H". iDestruct "H" as (x') "[% H]". subst. ss.
-    iApply back_ret. iModIntro. iApply "H".
-  Qed.
-
-  Lemma back_unwrapN_tgt
-        X
-        (Q: Any.t -> Any.t -> unit -> X -> iProp)
-        r g fuel f_src f_tgt st_src st_tgt x
-    :
-      bi_entails
-        (∀ x', ⌜x = Some x'⌝ -* Q st_src st_tgt tt x')
-        (back r g Q fuel f_src f_tgt (st_src, Ret tt) (st_tgt, unwrapN x)).
-  Proof.
-    iIntros "H". unfold unwrapN. destruct x.
-    { iApply back_ret. iModIntro. iApply "H". auto. }
-    { iApply back_triggerNB_tgt. auto. }
   Qed.
 End SIM.
 #[export] Hint Resolve _hsim_mon: paco.
