examples/mutsum/MutF01proofH.v
@@ -16,19 +16,13 @@ From ExtLib Require Import
      Structures.Maps
      Data.Map.FMapAList.
 
-Require Import HTactics ProofMode.
+Require Import HTactics ProofMode HSim IProofMode.
 
 Set Implicit Arguments.
 
 Local Open Scope nat_scope.
 
 
-(* TODO: HSim.v *)
-Require Import Red.
-Require Import IRed.
-
-Ltac hred_l := try (prw _red_gen 1 2 1 0).
-Ltac hred_r := try (prw _red_gen 1 1 1 0).
 
 Section SIMMODSEM.
 
@@ -39,50 +33,43 @@ Section SIMMODSEM.
   Let wf: unit -> Any.t -> Any.t -> iProp
     := (fun _ _ _ => (True: iProp)%I).
 
-  Require Import HSim.
+  Let top2_PreOrder: @PreOrder unit top2.
+  Proof. econs; eauto. Qed.
+  Local Existing Instance top2_PreOrder.
 
   Theorem correct: refines2 [MutF0.F] [MutF1.F].
   Proof.
     eapply adequacy_local2. econs; ss.
     i. econstructor 1 with (wf:=mk_wf wf) (le:=top2); et.
-    { ss. }
     2: { unfold wf. exists tt. econs; ss; red; uipropall. }
-    econs; ss. init.
-
-    harg. gfinal. right. eapply hsim_adequacy.
-    ginit. eapply back_init; [clear ACC|eapply ACC]. start_ipm_proof.
-
-    iDestruct "PRE" as "[% %]". des; clarify.
+    econs; ss. econs; ss.
+    apply back_fun_to_tgt; auto. i; ss.
+    iIntros "[INV %]". des. clarify.
     unfold fF, ccallU. ss. hred_r.
     iApply back_bind_right_pure. iApply back_assume_tgt. iSplit.
     { iPureIntro. eapply mut_max_intrange. auto. }
-
     destruct (dec (Z.of_nat x) 0%Z).
     - destruct x; ss. iApply back_apc. iExists None.
       hred_r. hred_l. iApply back_choose_src. iExists _.
-      iApply back_ret. iModIntro. iSplitL "INV"; eauto.
+      iApply back_ret. iSplitL "INV"; eauto.
     - destruct x; [ss|]. rewrite Nat2Z.inj_succ. hred_r.
       iApply back_apc. iExists (Some (10: Ord.t)).
       iApply back_call_pure; [|oauto|..].
-      { (* TODO: make lemmas *)
-        econs; ss.
-        { instantiate (1:=x). ss. eauto with ord_step. }
-        { i. iIntros "H". iModIntro. iExact "H". }
-        { i. iIntros "H". iModIntro. iExact "H". }
+      { eapply fn_has_spec_in_stb; eauto.
+        instantiate (1:=x). ss. eauto with ord_step.
       }
       iSplitL "INV".
-      { iModIntro. ss. iSplitR "INV"; eauto. iSplits; eauto.
+      { ss. iSplitR "INV"; eauto. iSplits; eauto.
         { iPureIntro.
           replace (Z.succ (Z.of_nat x) - 1)%Z with (Z.of_nat x) by lia.
           esplits; et.
         }
         { iPureIntro. lia. }
       }
-      ss. iIntros (st_src st_tgt ret_src ret_tgt) "[H0 %]".
-      des; clarify. iModIntro. hred_r. hred_l.
+      ss. iIntros (st_src0 st_tgt0 ret_src ret_tgt) "[H0 %]".
+      des; clarify. hred_r. hred_l.
       iApply back_choose_src. iExists _.
-      iApply back_ret. iModIntro. iSplitL "H0"; eauto. iSplits; eauto.
+      iApply back_ret. iSplitL "H0"; eauto. iSplits; eauto.
       iPureIntro. f_equal. f_equal. lia.
   Qed.
-
 End SIMMODSEM.
